### 12.3

Can we reduce the `factorial` base case argument from `0` to `-1`? If so, show the resulting procedure. If not, why not? 

***

Current definition:

~~~ scheme
(define (factorial n)
  (if (= n 0)
      1
      (* n (factorial (- n 1)))))
~~~

The following justification of why \\( 0! = 1 \\) was helpful to illustrate why it isnâ€™t possible to reduce the base case argument to `-1`:

\\( 4! = 4 \times 3 \times 2 \times 1 = 24 \\)

\\( 3! = \frac{4!} {4} = \frac{24} {4} = 6 \\)

\\( 2! = \frac{3!} {3} = \frac{6} {3} = 2 \\)

\\( 1! = \frac{2!} {2} = \frac{2} {1} = 1 \\)

\\( 0! = \frac{1!} {1} = \frac{1} {1} = 1 \\)

\\( -1! = \frac{0!}{0} = \frac{1}{0} = undefined \\)

The same logic applies to other negative numbers, and so the factorial of a negative number is undefined.
